Complete rewrite of Red_black_tree.v
Left insertion complete. Right insertion is symmetric, but not yet
completed.

	modified:   src/lib/Red_black_tree.v

src/lib/Red_black_tree.v
@@ -1,1664 +1,834 @@
 Require Import Core.
 Require Natural.
 Require List.
+Require Binary_search_tree.
 
 Import List.Notations.
 Import Equal.Notations.
 
 Set Implicit Arguments.
 Set Warnings "-extraction-opaque-accessed".
+Set Warnings "-extraction-inside-module".
+Unset Elimination Schemes.
 
 
-(* Invariant:
-   1. The black depth in both subtrees is the same.
-   2. A red parent has two black sons.
- *)
 
-
-(* Insertion:
-
-Rule: We always maintain the black-depth invariant, we temporarily violate the
-no-red-red invariant.
-
-Elementary case: Insert into an empty tree. A singleton red tree with two
-empty leaves. If we put the singleton red tree as a subtree into another node
-we might violate the no-red-red invariant in case that the parent node is
-red).
-
-Recursive case: Insert into a nonempty tree. We insert into the left or right
-son which might turn the son into a tree which has a no-red-red violation at
-the top.
-
-Insertion into a tree with a black root node never violates the no-red-red
-invariant because we can always rebalance and get a new tree with a red root.
-
-A tree with a red root node has two black sons. Insertion in one of the two
-might paint it red which causes a no-red-red violation.
-
-
-*)
-
-(****** Okasaki ***********)
-Module RB_Tree_nat.
-  Import Natural.
-  Inductive Color: Set := Red | Black.
-  Inductive Tree (A:Type): Type :=
-  | Leaf: Tree A
-  | Node: Color -> Tree A -> A -> Tree A -> Tree A.
-  Arguments Leaf [A].
-  Arguments Node [A] _ _ _ _.
-
-
-
-
-  Definition insert (x:nat) (a:Tree nat): Tree nat :=
-    let balance c t1 z t2 :=
-        let common a x b y c z d :=
-            Node Red (Node Black a x b) y (Node Black c z d)
-        in
-        match c with
-        | Red => Node c t1 z t2
-        | Black =>
-          match t1, t2 with
-          | Node Red (Node Red a x b) y c, t2 =>
-            common a x b y c z t2
-          | Node Red a x (Node Red b y c), t2 =>
-            common a x b y c z t2
-          | t1, Node Red (Node Red b y c) z d =>
-            common t1 x b y c z d
-          | t2, Node Red b y (Node Red c z d) =>
-            common t1 x b y c z d
-          | _, _ =>
-            Node c t1 z t2
-          end
-        end
-    in
-    let ins: Tree nat -> Tree nat :=
-        fix f a :=
-          match a with
-          | Leaf => Node Red Leaf x Leaf
-          | Node c t1 y t2 =>
-            match compare3 x y with
-            | Tristate.Left _ =>
-              balance c (f t1) y t2
-            | Tristate.Middle _ =>
-              Node c t1 y t2
-            | Tristate.Right _ =>
-              balance c t1 y (f t2)
-            end
-          end
-    in
-    let make_black a :=
-        match a with
-        | Leaf => Leaf
-        | Node c e t1 t2 => Node Black e t1 t2
-        end
-    in
-    make_black (ins a).
-
-End RB_Tree_nat.
-
-
-
-
-
-
-
-Module M1 (S0: SORTABLE).
-  Module S := Sortable_plus S0.
-  Import S.Notations.
-
-
-  Inductive Color: Set := Red | Black.
-
-  Definition is_Red (c:Color): Prop :=
-    match c with
-    | Red => True
-    | Black => False
-    end.
-
-  Definition is_Black (c:Color): Prop :=
-    match c with
-    | Red => False
-    | Black => True
-    end.
-
-  Theorem red_equal_black {A:Type} (eq:Red=Black): A.
-  Proof
-    ex_falso (Equal.use eq is_Red I).
-
-  Theorem black_equal_red {A:Type} (eq:Black=Red): A.
-  Proof
-    red_equal_black (Equal.flip eq).
-
-
-  Inductive tree: Type :=
-  | Leaf: tree
-  | Node: Color -> tree -> S.t -> tree -> tree.
-
-  Definition is_Node (t:tree): Prop :=
-    match t with
-    | Leaf => False
-    | Node _ _ _ _ => True
-    end.
-
-  Definition is_node (t:tree): {is_Node t} + {~ is_Node t} :=
-    match t with
-    | Leaf => right (fun nd:False => ex_falso nd)
-    | Node c t1 x t2 =>
-      left I
-    end.
-
-  Definition is_Node_red (t:tree): Prop :=
-    match t with
-    | Leaf => False
-    | Node c _ _ _ => is_Red c
-    end.
-
-  Definition is_Node_black (t:tree): Prop :=
-    match t with
-    | Leaf => False
-    | Node c _ _ _ => is_Black c
-    end.
-
-
-  Definition color (t:tree): Color :=
-    match t with
-    | Leaf => Black
-    | Node c _ _ _ => c
-    end.
-
-  Theorem node_equal_leaf
-          {A:Type} {c:Color} {x:S.t} {u v:tree}
-          (eq:Node c u x v = Leaf): A.
-  Proof
-    ex_falso (Equal.use eq is_Node I).
-
-  Theorem leaf_equal_node
-          {A:Type} {c:Color} {x:S.t} {u v:tree}
-          (eq:Leaf = Node c u x v): A.
-  Proof
-    node_equal_leaf (Equal.flip eq).
-
-
-  Theorem leaf_ne_node:
-    forall (c:Color) (x:S.t) (u v:tree),
-      Leaf <> Node c u x v.
-  Proof.
-    intros c x u v eq. inversion eq.
-  Qed.
-
-  Theorem node_injective:
-    forall (c1 c2:Color) (x1 x2:S.t) (t1 t2 u1 u2:tree),
-      Node c1 t1 x1 u1 = Node c2 t2 x2 u2 ->
-      c1 = c2 /\ x1 = x2 /\ t1 = t2 /\ u1 = u2.
-  Proof.
-    intros c1 c2 x1 x2 t1 t2 u1 u2 eq.
-    inversion eq.
-    split. reflexivity. split. reflexivity. split;reflexivity.
-  Qed.
-
-  Theorem node_injective2:
-    forall (c1 c2:Color) (x1 x2:S.t) (t1 t2 u1 u2:tree),
-      Node c1 t1 x1 u1 = Node c2 t2 x2 u2 ->
-      c1 = c2 /\ x1 = x2 /\ t1 = t2 /\ u1 = u2.
-  Proof.
-    refine(
-        let elem d t :=
-            match t with
-            | Leaf => d
-            | Node c t x u => x
-            end in
-        let left d t :=
-            match t with
-            | Leaf => d
-            | Node c t x u => t
-            end in
-        let right d t :=
-            match t with
-            | Leaf => d
-            | Node c t x u => u
-            end in
-        fun c1 c2 x1 x2 t1 t2 u1 u2 eq =>
-          let eqc: x1 = x2 := Equal.inject eq (elem x1) in
-          And.make4
-            (Equal.inject eq color)
-            (Equal.inject eq (elem x1))
-            (Equal.inject eq (left t1))
-            (Equal.inject eq (right t2))
-      ).
-  Qed.
-
-
-  Theorem use_node_equal:
-    forall {A:Prop} (c1 c2:Color) (x1 x2:S.t) (t1 t2 u1 u2:tree),
-      Node c1 t1 x1 u1 = Node c2 t2 x2 u2 ->
-      (c1=c2 -> x1=x2 -> t1=t2 -> u1=u2->A)
-      -> A.
-  Proof.
-    refine(
-        fun A c1 c2 x1 x2 t1 t2 u1 u2 eq P =>
-          let elem t :=
-              match t with
-              | Leaf => x1
-              | Node c t x u => x
-              end in
-          let left t :=
-              match t with
-              | Leaf => t1
-              | Node c t x u => t
-              end in
-          let right t :=
-              match t with
-              | Leaf => t2
-              | Node c t x u => u
-              end in
-          P (Equal.inject eq color)
-            (Equal.inject eq elem)
-            (Equal.inject eq left)
-            (Equal.inject eq right)
-      ).
-  Qed.
-
-
-
-
-  Module Inorder.
-    Inductive R: tree -> list S.t -> Prop :=
-    | leaf: R Leaf []
-    | node:
-        forall c t1 l1 x t2 l2,
-          R t1 l1 ->
-          R t2 l2 ->
-          R (Node c t1 x t2) (l1 ++ x :: l2).
-
-    Fixpoint make (t:tree): list S.t :=
-      match t with
-      | Leaf => []
-      | Node c t x u => make t ++ x :: (make u)
-      end.
-
-    Theorem list_to_rel:
-      forall (t:tree) (l:list S.t),
-        l = make t ->
-        R t l.
-    Proof
-      fix f t :=
-      match t with
-      | Leaf =>
-        fun l (eq: l = make Leaf) =>
-          let p := leaf in
-          Equal.use
-            (Equal.flip eq)
-            (fun l => R Leaf l)
-            leaf
-      | Node c u x v =>
-        fun l (eq: l = make (Node c u x v)) =>
-          Equal.use
-            (Equal.flip eq)
-            (fun l => R _ l)
-            (node c x (f u (make u) eq_refl) (f v (make v) eq_refl))
-      end.
-
-
-    Theorem rel_to_list:
-      forall (t:tree) (l:list S.t),
-        R t l ->
-        l = make t.
-    Proof
-      fix f t l r {struct r}:=
-      match r with
-      | leaf =>
-        eq_refl: [] = make Leaf
-      | node c x r1 r2 =>
-        Equal.use2
-           (Equal.flip (f _ _ r1) : make _ = _)
-           (Equal.flip (f _ _ r2) : make _ = _)
-           (fun a b => a ++ x :: b = _)
-           eq_refl
-        : _ ++ x :: _ = make (Node c _ x _)
-      end.
-
-
-    Theorem make_correct (t:tree): R t (make t).
-    Proof
-      (fix f t :=
-      match t with
-      | Leaf => leaf:R Leaf (make Leaf)
-      | Node c t x u =>
-        node c x (f t) (f u) : R _ (make (Node c t x u))
-      end) t.
-
-    Theorem unique:
-      forall (t:tree) (a b:list S.t),
-        R t a ->
-        R t b ->
-        a = b.
-    Proof
-      fun t a b r1 r2 =>
-        let p := rel_to_list r1 in
-        Equal.join (rel_to_list r1) (Equal.flip (rel_to_list r2)).
-  End Inorder.
-
-
-
-
-  Inductive Domain: tree -> S.t -> Prop :=
-  | dom_singleton:
-      forall c x,
-        Domain (Node c Leaf x Leaf) x
-  | dom_left:
-      forall x c t y u,
-        Domain t x -> Domain (Node c t y u) x
-  | dom_right:
-      forall x c t y u,
-        Domain u x -> Domain (Node c t y u) x
-  | dom_root:
-      forall x c t y u,
-        x = y  -> Domain (Node c t y u) x.
-
-
-  Inductive Red_black: nat -> Color -> tree -> Prop :=
-  | rb_leaf: Red_black 0 Black Leaf
-  | rb_red:
-      forall n t1 x t2,
-        Red_black n Black t1 ->
-        Red_black n Black t2 ->
-        Red_black n Red (Node Red t1 x t2)
-  | rb_black:
-      forall n c1 t1 x c2 t2,
-        Red_black n c1 t1 ->
-        Red_black n c2 t2 ->
-        Red_black (S n) Black (Node Black t1 x t2).
-
-  Theorem rb_inv_leaf:
-    forall (h:nat) (c:Color),
-      Red_black h c Leaf ->
-      h = 0 /\ c = Black.
-  Proof.
-    refine(
-        fun h c rb =>
-          _
-      ).
-    inversion rb.
-    split; reflexivity.
-  Qed.
-
-  Theorem rb_inv_color:
-    forall (h:nat) (c:Color) (t:tree),
-      Red_black h c t ->
-      Red_black h (color t) t.
-  Proof.
-    intros h c t rb.
-    inversion rb as [ | | n c1 t1 x c2 t2 ].
-    - apply rb_leaf.
-    - simpl. apply rb_red;assumption.
-    - simpl. apply rb_black with (c1:=c1) (c2:=c2);assumption.
-  Qed.
-
-  Theorem use_rb_leaf:
-    forall (h:nat) (c:Color),
-      Red_black h c Leaf ->
-      forall (P:nat->Color->Prop),
-        P 0 Black ->
-        P h c.
-  Proof.
-    refine(
-      fun h c inv =>
-        _
-      ).
-    inversion inv. intros P p. assumption.
-  Qed.
-
-
-  Theorem use_rb_red:
-    forall (h:nat) (x:S.t) (t1 t2:tree),
-      Red_black h Red (Node Red t1 x t2) ->
-      forall P:nat->tree->S.t->tree->Prop,
-        (Red_black h Black t1 -> Red_black h Black t2 -> P h t1 x t2) ->
-        P h t1 x t2.
-  Proof.
-    refine (
-        fun h x t1 t2 inv =>
-          _
-      ).
-    inversion inv. intros P impl. apply impl; assumption.
-  Qed.
-
-
-  Theorem use_rb_black:
-    forall (h:nat) (x:S.t) (t1 t2:tree),
-      Red_black h Black (Node Black t1 x t2) ->
-      forall (P:nat->tree->S.t->tree->Prop),
-        (
-         Red_black (pred h) (color t1) t1 ->
-         Red_black (pred h) (color t2) t2 ->
-         P h t1 x t2) ->
-        P h t1 x t2.
-  Proof.
-    refine (
-        fun h x t1 t2 inv =>
-          _
-      ).
-    inversion inv as [| | n d1 u1 y d2 u2 rb1 rb2 ].
-    intros P impl. apply impl.
-    - apply rb_inv_color with (c:=d1);assumption.
-    - apply rb_inv_color with (c:=d2);assumption.
-  Qed.
-
-  Theorem use_rb_black2:
-    forall (h:nat) (c:Color) (x:S.t) (t1 t2:tree),
-      Red_black h c (Node Black t1 x t2) ->
-      forall (P:nat->Color->tree->S.t->tree->Prop),
-        (
-         Red_black (pred h) (color t1) t1 ->
-         Red_black (pred h) (color t2) t2 ->
-         P h Black t1 x t2) ->
-        P h c t1 x t2.
-  Proof.
-    refine (
-        fun h c x t1 t2 inv =>
-          _
-      ).
-    inversion inv as [| | n d1 u1 y d2 u2 rb1 rb2 ].
-    intros P impl. apply impl.
-    - apply rb_inv_color with (c:=d1);assumption.
-    - apply rb_inv_color with (c:=d2);assumption.
-  Qed.
-
-
-
-  Theorem height_unique0: (* see below 'height_unique' *)
-    forall {h1 h2:nat} {c1 c2:Color} {t1 t2:tree},
-      Red_black h1 c1 t1 ->
-      Red_black h2 c2 t2 ->
-      t1 = t2 ->
-      h1 = h2.
-  Proof
-    fix f h1 h2 c1 c2 t1 t2 rb1:=
-    match rb1 with
-    | rb_leaf =>
-      fun rb2 =>
-        match rb2 with
-        | rb_leaf =>
-          fun _ => eq_refl
-        | rb_red _ _ _  =>
-          fun eq => leaf_equal_node eq
-        | rb_black _ _ _ =>
-          fun eq => leaf_equal_node eq
-        end
-    | rb_red _ rbu1 _ =>
-      fun rb2 =>
-        match rb2 with
-        | rb_leaf => fun eq => node_equal_leaf eq
-        | rb_red _ rbu2 _ =>
-          fun eq =>
-            use_node_equal
-              eq
-              (fun _ _ equ1 _ =>
-                 f _ _ _ _ _ _ rbu1 rbu2 equ1)
-        | rb_black _ rbu2 _ =>
-          fun eq =>
-            use_node_equal
-              eq
-              (fun rbeq => red_equal_black rbeq)
-        end
-    | rb_black x1 rbu1 rbv1 =>
-      fun rb2 =>
-        match rb2 with
-        | rb_leaf =>  fun eq => node_equal_leaf eq
-        | rb_red _ _ _ =>
-          fun eq =>
-            use_node_equal
-              eq
-              (fun breq => black_equal_red breq)
-        | rb_black _ rbu2 _ =>
-          fun eq =>
-            use_node_equal
-              eq
-              (fun _ _ equ1 _ =>
-                 Equal.inject
-                   (f _ _ _ _ _ _ rbu1 rbu2 equ1)
-                   S
-              )
-        end
-    end.
-
-
-  Fixpoint black_height (t:tree): nat :=
-    match t with
-    | Leaf => 0
-    | Node Red t1 x t2 => black_height t1
-    | Node Black t1 x t2 => S (black_height t1)
-    end.
-
-  Theorem black_height_correct:
-    forall (h:nat) (c:Color) (t:tree),
-      Red_black h c t -> h = black_height t.
-  Proof
-    fix f h c t rb :=
-      match rb with
-      | rb_leaf => eq_refl
-      | rb_red x rb1 rb2   => f _ _ _ rb1
-      | rb_black x rb1 rb2 => Equal.inject (f _ _ _ rb1) S
-      end.
-
-  Theorem height_unique:
-    forall {h1 h2:nat} {c1 c2:Color} {t:tree},
-      Red_black h1 c1 t ->
-      Red_black h2 c2 t ->
-      h1 = h2.
-  Proof
-    fun h1 h2 c1 c2 t rb1 rb2 =>
-      Equal.join
-        (black_height_correct rb1)
-        (Equal.flip (black_height_correct rb2)).
-
-
-  Theorem color_correct {h:nat} {c:Color} {t:tree} (rb:Red_black h c t)
-    : c = color t.
-  Proof
-      match rb in Red_black h c t return c = color t with
-      | rb_leaf => eq_refl
-      | rb_red x rb1 rb2 => eq_refl
-      | rb_black x rb1 rb2 => eq_refl
-      end.
-
-  Theorem color_unique {h1 h2:nat} {c1 c2:Color} {t:tree}
-      (rb1:Red_black h1 c1 t) (rb2:Red_black h2 c2 t): c1 = c2.
-  Proof
-    Equal.join (color_correct rb1) (Equal.flip (color_correct rb2)).
-
-
-  Theorem generalize_height_color:
-    forall  (h:nat) (c:Color) (t:tree) (P:nat->Color->Prop),
-      Red_black h c t ->
-      P h c ->
-      forall h c,
-        Red_black h c t -> P h c.
-  Proof
-    fun h c t P rb p h1 c1 rb1 =>
-      Equal.use2
-        (height_unique rb rb1:h=h1)
-        (color_unique  rb rb1:c=c1)
-        P p.
-
-  Theorem generalize_height:
-    forall  (h:nat) (c:Color) (t:tree) (P:nat->Prop),
-      Red_black h c t ->
-      P h ->
-      forall h,
-        Red_black h c t -> P h.
-  Proof
-    fun h c t P rb p h1 rb1 =>
-      @generalize_height_color
-        h c t
-        (fun h c => P h)
-        rb p h1 c rb1.
-
-  Definition Same_black (t1 t2:tree): Prop :=
-    black_height t1 = black_height t2.
-
-  Definition is_Red_black (t:tree): Prop :=
-    exists h, Red_black h (color t) t.
-
-  Theorem use_node_red_black:
-    forall (A:Prop) (c:Color) (x:S.t) (u v:tree),
-      is_Red_black (Node c u x v) ->
-      (is_Red_black u -> is_Red_black v -> A) ->
-      A.
-  Proof
-    fun A c x u v =>
-      match c with
-      | Red =>
-        fun rb =>
-          Exist.use
-            rb
-            (fun h (red:Red_black h Red (Node Red u x v)) f =>
-               use_rb_red
-                 red
-                 (fun h u x v => A)
-                 (fun rb1 rb2 =>
-                    let eqc1 := color_correct rb1 in
-                    let eqc2 := color_correct rb2 in
-                    let p1 := Equal.use eqc1 (fun c => Red_black _ c _) rb1 in
-                    let p2 := Equal.use eqc2 (fun c => Red_black _ c _) rb2 in
-                    f (ex_intro _ h p1) (ex_intro _ h p2)
-                 )
-            )
-      | Black =>
-        fun rb =>
-          Exist.use
-            rb
-            (fun h (blck:Red_black h Black (Node Black u x v)) f =>
-               use_rb_black
-                 blck
-                 (fun h u x v => A)
-                 (fun rb1 rb2 =>
-                    let eqc1 := color_correct rb1 in
-                    let eqc2 := color_correct rb2 in
-                    let p1 := Equal.use eqc1 (fun c => Red_black _ c _) rb1 in
-                    let p2 := Equal.use eqc2 (fun c => Red_black _ c _) rb2 in
-                    f (ex_intro _ (pred h) p1) (ex_intro _ (pred h) p2)
-                 )
-            )
-
-      end.
-
-  Theorem left_son_red_black:
-    forall (c:Color) (x:S.t) (u v:tree),
-      is_Red_black (Node c u x v) ->
-      is_Red_black u.
-  Proof
-    fun c x u v rb =>
-    use_node_red_black rb (fun rb1 rb2 => rb1).
-
-  Theorem right_son_red_black:
-    forall (c:Color) (x:S.t) (u v:tree),
-      is_Red_black (Node c u x v) ->
-      is_Red_black v.
-  Proof
-    fun c x u v rb =>
-    use_node_red_black rb (fun rb1 rb2 => rb2).
-
-
-
-
-
-
-  Inductive RB_nearly0: nat -> tree -> Prop :=
-    nearly:
-      forall n c1 t1 x c2 t2 c3,
-        Red_black n c1 t1 ->
-        Red_black n c2 t2 ->
-        RB_nearly0 n (Node c3 t1 x t2).
-
-  Inductive RB_nearly: nat -> tree -> Prop :=
-    rb_nearly:
-      forall n c1 t1 x c2 t2,
-        Red_black n c1 t1 ->
-        Red_black n c2 t2 ->
-        RB_nearly n (Node Red t1 x t2).
-
-
-
-  Theorem singleton_nearly:
-    forall (c:Color) (x:S.t), RB_nearly0 0 (Node c Leaf x Leaf).
-  Proof
-        fun c x =>
-          let t := Node c Leaf x Leaf in
-          nearly x c rb_leaf rb_leaf.
-
-  Theorem use_rb_nearly_leaf:
-    forall (h:nat),
-      RB_nearly0 h Leaf ->
-      h = 0.
-  Proof.
-    intros h rbn.
-    inversion rbn.
-  Qed.
-
-  Definition is_Nearly (t:tree): Prop :=
-    exists h, RB_nearly0 h t.
-
-  Inductive Rotation: tree -> tree -> Prop :=
-  | rot_leaf:
-      Rotation Leaf Leaf
-  | rot_left:
-      forall c1 c2 c3 c4 a x b y c,
-        Rotation
-          (Node c1 a x (Node c2 b y c))
-          (Node c3 (Node c4 a x b) y c)
-  | rot_right:
-      forall c1 c2 c3 c4 a x b y c,
-        Rotation
-          (Node c1 (Node c2 a x b) y c)
-          (Node c3 a x (Node c4 b y c))
-  | rot_node:
-      forall c1 c2 x t11 t12 t21 t22,
-        Rotation t11 t12 ->
-        Rotation t21 t22 ->
-        Rotation (Node c1 t11 x t21) (Node c2 t12 x t22)
-  | rot_trans:
-      forall t1 t2 t3,
-        Rotation t1 t2 -> Rotation t2 t3 -> Rotation t1 t3.
-
-  Theorem rotation_reflexive:
-    forall (t:tree), Rotation t t.
-  Proof
-    fix f t :=
-    match t with
-    | Leaf => rot_leaf
-    | Node c t1 x t2 =>
-      let r1 := f t1 in
-      let r2 := f t2 in
-      rot_node c c x r1 r2
-    end.
-
-  Theorem rotation_to_node:
-    forall (u v:tree),
-      Rotation u v ->
-      is_Node u ->
-      is_Node v.
-  Proof
-    fix f u v rot :=
-    match rot with
-    | rot_leaf =>
-    fun nd => ex_falso nd
-    | @rot_left c1 c2 c3 c4 a x b y c =>
-      fun nd => I
-    | @rot_right c1 c2 c3 c4 a x b y c =>
-      fun nd => I
-    | @rot_node c1 c2 x t1 t2 u1 u2 rt ru =>
-      fun nd => I
-    | @rot_trans u v w ruv rvw =>
-      fun ndu => f v w rvw (f u v ruv ndu)
-    end.
-
-
-  (** Rotation keeps the inorder sequence. The proof recurses over all
-  constructors of a rotation.
-
-  The left and right rotation uses the associativity of list append.
-
-  The node construction uses the fact that rotations of the sons keep their
-  inorder sequence. Using this we can transform an inorder sequence of the
-  node before the rotation into the same inorder sequence of the node after
-  rotation.
-
-  Transitivity is a simple application of two rotations keeping the inorder
-  sequence.*)
-  Theorem rotation_inorder:
-    forall (t u:tree),
-      Rotation t u ->
-      forall l,
-        Inorder.R t l ->
-        Inorder.R u l.
-  Proof
-    fix f t u rot:=
-    match rot with
-    | rot_leaf =>
-      fun l ord => ord
-    | @rot_left c1 c2 c3 c4 a x b y c =>
-      fun l inord =>
-        let t := Node c1 a x (Node c2 b y c) in
-        let u := Node c3 (Node c4 a x b) y c in
-        let eq: l = Inorder.make u :=
-            Equal.join
-               (Inorder.rel_to_list inord
-                : l = _ ++ x :: _ ++ y :: _)
-               (Equal.flip (List.app_associative _ (x::_) (y::_))
-                : _ = (_ ++ x :: _) ++ y :: _)
-        in
-        Inorder.list_to_rel u eq
-        : Inorder.R u l
-    | @rot_right c1 c2 c3 c4 a x b y c =>
-      fun l inord =>
-        let t := Node c1 (Node c2 a x b) y c in
-        let u := Node c3 a x (Node c4 b y c) in
-        let eq : l = Inorder.make u :=
-            Equal.join
-               (Inorder.rel_to_list inord: l = (_ ++ x :: _) ++ y :: _)
-               (List.app_associative _ (x::_) (y::_)
-                : _ = _ ++ x :: _ ++ y :: _)
-        in
-        Inorder.list_to_rel u eq: Inorder.R u l
-    | @rot_node c1 c2 x t1 t2 u1 u2 rt ru =>
-      fun l ord =>
-        let t := Node c1 t1 x u1 in
-        let u := Node c2 t2 x u2 in
-        let eq: l = Inorder.make u :=
-            (equality_chain:
-               (Inorder.rel_to_list ord
-                : l = Inorder.make t1 ++ x :: Inorder.make u1),
-               (
-                Equal.use2
-                  (Inorder.rel_to_list (f _ _ rt _ (Inorder.make_correct t1))
-                   : Inorder.make t1 = Inorder.make t2)
-                  (Inorder.rel_to_list (f _ _ ru _ (Inorder.make_correct u1))
-                   : Inorder.make u1 = Inorder.make u2)
-                  (fun a b => _ = a ++ x :: b)
-                  eq_refl
-                : _ = Inorder.make t2 ++ x :: Inorder.make u2)
-            )
-        in
-        Inorder.list_to_rel u eq : Inorder.R u l
-    | @rot_trans u v w ruv rvw =>
-      fun l ord_ul =>
-        f v w rvw l (f u v ruv  l ord_ul)
-    end.
-
-
-
-
-
-
-  Inductive Bounded: S.t -> tree -> S.t -> Prop :=
-  | leaf_bounded:
-      forall lo hi,
-        lo <= hi ->
-        Bounded lo Leaf hi
-  | node_bounded:
-      forall lo t1 x t2 hi c,
-        Bounded lo t1 x ->
-        Bounded x t2 hi ->
-        Bounded lo (Node c t1 x t2) hi.
-
-  Theorem use_leaf_bounded:
-    forall (lo hi:S.t),
-      Bounded lo Leaf hi ->
-      forall (A:Prop) (P:lo<=hi->A), A.
-  Proof.
-    intros lo hi b.
-    inversion b. intros A impl. apply impl. assumption.
-  Qed.
-
-  Theorem use_node_bounded0:
-    forall {A:Prop} (c:Color) (lo x hi:S.t) (t1 t2:tree),
-      Bounded lo (Node c t1 x t2) hi ->
-      (Bounded lo t1 x -> Bounded x t2 hi -> A) -> A.
-  Proof.
-    intros A c lo x hi t1 t2 b.
-    inversion b.
-    intros impl. apply impl;assumption.
-  Qed.
-
-
-  Theorem use_node_bounded:
-    forall {A:Prop} (c:Color) (lo x hi:S.t) (t1 t2:tree),
-      Bounded lo (Node c t1 x t2) hi ->
-      (Bounded lo t1 x -> Bounded x t2 hi -> A) -> A.
-  Proof
-    fun A c lo x hi t1 t2 b =>
-      let lemma lo t hi:
-            Bounded lo t hi ->
-            forall c t1 x t2,
-              t = Node c t1 x t2 ->
-              (Bounded lo t1 x -> Bounded x t2 hi -> A) -> A :=
-          fun b =>
-            match b with
-            | @leaf_bounded lo hi le =>
-              fun c t1 x t2 eq => leaf_equal_node eq
-            | @node_bounded lo t1 x t2 hi c b1 b2 =>
-              fun c0 u1 y u2 eq =>
-                use_node_equal
-                  eq
-                  (fun ceq xeq t1eq t2eq f =>
-                     f (Equal.use2 xeq t1eq (fun x t => Bounded lo t x) b1)
-                       (Equal.use2 xeq t2eq (fun x t => Bounded x t hi) b2)
-                  )
-            end
-      in
-      lemma lo (Node c t1 x t2) hi b c t1 x t2 eq_refl.
-
-
-
-  Theorem bounds_le:
-    forall (lo hi:S.t) (t:tree),
-      Bounded lo t hi ->
-      lo <= hi.
-  Proof
-    fix f lo hi t bnd:=
-      match bnd with
-      | leaf_bounded le => le
-      | @node_bounded lo t1 x t2 hi c b1 b2 =>
-        S.transitive
-          (f lo x t1 b1)
-          (f x hi t2 b2)
-      end.
-
-
-  Theorem bounded_left_transitive:
-    forall (x lo hi:S.t) (t:tree),
-      Bounded lo t hi ->
-      x <= lo ->
-      Bounded x t hi.
-  Proof
-    fix f x lo hi t bnd:=
-      match bnd with
-      | leaf_bounded le_lo_hi =>
-        fun le_x_lo =>
-          leaf_bounded (S.transitive le_x_lo le_lo_hi)
-      | node_bounded c bnd1 bnd2 =>
-        fun le_x_lo1 =>
-          node_bounded
-            c (f _ _ _ _ bnd1 le_x_lo1)
-            bnd2
-      end.
-
-  Theorem bounded_right_transitive:
-    forall (x lo hi:S.t) (t:tree),
-      Bounded lo t hi ->
-      hi <= x ->
-      Bounded lo t x.
-  Proof
-    fix f x lo hi t bnd:=
-      match bnd with
-      | leaf_bounded le_lo_hi =>
-        fun le_hi_x =>
-          leaf_bounded (S.transitive le_lo_hi le_hi_x)
-      | node_bounded c bnd1 bnd2 =>
-        fun le_hi2_x =>
-          node_bounded
-            c bnd1
-            (f _ _ _ _ bnd2 le_hi2_x)
-      end.
-
-  Theorem rotation_bounded:
-    forall (t u:tree),
-      Rotation t u ->
-      forall (lo hi:S.t),
-        Bounded lo t hi ->
-        Bounded lo u hi.
-  Proof
-    fix f t u rot :=
-    match rot with
-    | @rot_left c1 c2 c3 c4 a x b y c =>
-      fun lo hi bnd =>
-        use_node_bounded
-          bnd
-          (fun bnd1 bnd2 =>
-             use_node_bounded
-               bnd2
-               (fun bnd2a bnd2b =>
-                  node_bounded c3 (node_bounded c4 bnd1 bnd2a) bnd2b
-               )
-          )
-    | @rot_right c1 c2 c3 c4 a x b y c =>
-      fun lo hi bnd =>
-        use_node_bounded
-          bnd
-          (fun bnd1 bnd2 =>
-             use_node_bounded
-               bnd1
-               (fun bnd1a bnd1b =>
-                  node_bounded c3 bnd1a (node_bounded c4 bnd1b bnd2)
-               )
-          )
-    | rot_leaf =>
-      fun _ _ b => b
-    | @rot_node c1 c2 x u1 u2 v1 v2 ru rv =>
-      fun lo hi bnd =>
-        use_node_bounded
-          bnd
-          (fun bnd1 bnd2 =>
-             let b1new := f u1 u2 ru lo x bnd1 in
-             let b2new := f v1 v2 rv x hi bnd2 in
-             node_bounded c2 b1new b2new
-          )
-    | @rot_trans t u v tu uv =>
-      fun lo hi bnd =>
-        f u v uv lo hi (f t u tu lo hi bnd)
-    end.
-
-  Definition Sorted (t:tree): Prop :=
-    exists lo hi, Bounded lo t hi.
-
-  Theorem use_node_sorted:
-    forall (A:Prop) (c:Color) (x:S.t) (u v:tree),
-      Sorted (Node c u x v) ->
-      (Sorted u -> Sorted v -> A) ->
-      A.
-  Proof
-    fun A c x u v s =>
-      Exist.use2
-        s
-        (fun lo hi b =>
-           use_node_bounded
-             b
-             (fun b1 b2 =>
-                fun f =>
-                  f (Exist.make2 b1)
-                    (Exist.make2 b2))).
-
-  Theorem left_son_sorted:
-    forall (c:Color) (x:S.t) (u v:tree),
-      Sorted (Node c u x v) ->
-      Sorted u.
-  Proof
-    fun c x u v s =>
-      use_node_sorted
-        s (fun s1 s2 => s1).
-
-
-  Theorem right_son_sorted:
-    forall (c:Color) (x:S.t) (u v:tree),
-      Sorted (Node c u x v) ->
-      Sorted v.
-  Proof
-    fun c x u v s =>
-      use_node_sorted
-        s (fun s1 s2 => s2).
-
-
-
-  Definition RB_sorted (t:tree): Prop := is_Red_black t /\ Sorted t.
-
-  Definition RB_nearly_sorted (t:tree): Prop := is_Nearly t /\ Sorted t.
-
-  Theorem singleton_sorted:
-    forall (c:Color) (x:S.t), Sorted (Node c Leaf x Leaf).
-  Proof
-    fun c x =>
-      let le_xx: x <= x := S.reflexive x in
-      let leafb: Bounded x Leaf x := leaf_bounded le_xx in
-      let t := Node c Leaf x Leaf in
-      let b: Bounded x t x :=
-          node_bounded c leafb leafb
-      in
-      Exist.make2 b.
-
-
-  Definition Lower_bound (t:tree) (lo:S.t): Prop :=
-    exists hi, Bounded lo t hi.
-
-  Definition Upper_bound (t:tree) (hi:S.t): Prop :=
-    exists lo, Bounded lo t hi.
-
-  Theorem lower_bound_to_sorted:
-    forall (t:tree) (lo:S.t),
-      Lower_bound t lo ->
-      Sorted t.
-  Proof
-    fun t lo lb =>
-      Exist.use lb (fun hi bnd => Exist.make2 bnd).
-
-  Theorem upper_bound_to_sorted:
-    forall (t:tree) (hi:S.t),
-      Upper_bound t hi ->
-      Sorted t.
-  Proof
-    fun t hi hb =>
-      Exist.use hb (fun ls bnd => Exist.make2 bnd).
-
-
-  Theorem sons_bounded:
-    forall (c:Color) (lo hi x:S.t) (u v:tree),
-      Bounded lo (Node c u x v) hi ->
-      Bounded lo u x /\ Bounded x v hi.
-  Proof
-    fun c lo hi x u v b =>
-      use_node_bounded
-        b
-        (fun b1 b2 => conj b1 b2).
-
-  (*
-  Theorem sons_sorted:
-    forall (c:Color) (x:S.t) (t u:tree),
-      Sorted (Node c t x u) ->
-      Sorted t /\ Sorted u.
-  Proof
-    fun c x t u sort =>
-      match is_node (Node c t x u) with
-      | left p =>
-        Exist.use2
-          (sort p)
-          (fun lo hi b =>
-             And.use
-               (sons_bounded b)
-               (fun b1 b2 =>
-                  (conj
-                     (fun _ => Exist.make2 b1)
-                     (fun _ => Exist.make2 b2) )))
-      | right p => ex_falso (p I)
-      end.
-*)
-  Theorem lower_upper_to_bounded:
-    forall (lo hi:S.t) (t:tree),
-      Lower_bound t lo ->
-      Upper_bound t hi ->
-      Bounded lo t hi.
-  Proof.
-    refine (
-        fun lo hi t lb ub =>
-          Exist.use
-            lb
-            (fun x1 (b1: Bounded lo t x1) =>
-               Exist.use
-                 ub
-                 (fun x2 (b2: Bounded x2 t hi) =>
-                    _))
-      ).
-
-
-
-  Theorem node_sorted:
-    forall (c:Color) (t1:tree) (x:S.t) (t2:tree),
-      Upper_bound t1 x ->
-      Lower_bound t2 x ->
-      Sorted (Node c t1 x t2).
-  Proof
-    fun c t1 x t2 hb lb =>
-      let le_xx: x <= x := S.reflexive x in
-      Exist.use
-        hb
-        (fun lo1 bnd1 =>
-           Exist.use
-             lb
-             (fun hi2 bnd2 =>
-                Exist.make2 (node_bounded c bnd1 bnd2)
-             )
-        ).
-
-
-
-
-  Theorem domain_bounded:
-    forall (z:S.t) (t:tree),
-      Domain t z ->
-      forall (lo hi:S.t),
-        Bounded lo t hi ->
-        lo <= z /\ z <= hi.
-  Proof.
-    refine(
-        fix f z t dom :=
-          match dom with
-          | @dom_singleton c x =>
-            fun lo hi b =>
-              And.use
-                (sons_bounded b)
-                (fun b1 b2 =>
-                   conj (bounds_le b1) (bounds_le b2))
-          | @dom_left x c t y u dom =>
-            fun lo hi b =>
-              And.use
-                (sons_bounded b)
-                (fun b1 b2 =>
-                   And.use
-                     (f x t dom lo y b1)
-                     (fun p1 p2 =>
-                        conj
-                          p1
-                          (S.transitive p2 (bounds_le b2))
-                     )
-                )
-          | @dom_right x c t y u dom =>
-            fun lo hi b =>
-              And.use
-                (sons_bounded b)
-                (fun b1 b2 =>
-                   And.use
-                     (f x u dom y hi b2)
-                     (fun p1 p2 =>
-                        conj
-                          (S.transitive (bounds_le b1) p1)
-                          p2
-                     )
-                )
-          | @dom_root x c t y u eq =>
-            fun lo hi b =>
-              And.use
-                (sons_bounded b)
-                (fun b1 b2 =>
-                   Equal.rewrite_bwd
-                     (fun z => lo <= z /\ z <= hi)
-                     eq
-                     (conj (bounds_le b1) (bounds_le b2))
-                )
-          end
-      ).
-  Qed.
-
-
-
-
-
-
-  Inductive Inserted: S.t -> tree -> tree -> Prop :=
-  | ins_leaf:
-      forall c x, Inserted x Leaf (Node c Leaf x Leaf)
-  | ins_left:
-      forall c x y t1 t1new t2,
-        x <= y ->
-        Inserted x t1 t1new ->
-        Inserted x (Node c t1 y t2) (Node c t1new y t2)
-  | ins_right:
-      forall c x y t1 t2 t2new,
-        y <= x ->
-        Inserted x t2 t2new ->
-        Inserted x (Node c t1 y t2) (Node c t1 y t2new)
-  | ins_replace:
-      forall c x y t1 t2,
-        S.Equivalent x y ->
-        Inserted x (Node c t1 y t2) (Node c t1 x t2)
-  | ins_rotation:
-      forall x t1 t2 t3,
-        Inserted x t1 t2 ->
-        Rotation t2 t3 ->
-        Inserted x t1 t3.
-
-
-  Theorem inserted_to_node:
-    forall (x:S.t) (u v:tree),
-      Inserted x u v ->
-      is_Node v.
-  Proof
-    fix f x u v ins :=
-    match ins with
-    | ins_leaf c x =>
-      I
-    | @ins_left c x y t1 t1new t2 xy ins =>
-      I
-    | @ins_right c x y t1 t2 t2new yx ins =>
-      I
-    | @ins_replace c x y t1 t2 eqv =>
-      I
-    | @ins_rotation x t1 t2 t3 ins rot =>
-      rotation_to_node rot (f x t1 t2 ins)
-    end.
-
-
-  Theorem inserted_to_bounded:
-    forall (x:S.t) (t1 t2:tree),
-      Inserted x t1 t2 ->
-      forall lo hi,
-        lo <= x ->
-        x <= hi ->
-        Bounded lo t1 hi ->
-        Bounded lo t2 hi.
-  Proof
-    fix f x t1 t2 ins :=
-    match ins with
-    | ins_leaf c x =>
-      fun lo hi lox xhi b =>
-        node_bounded c (leaf_bounded lox) (leaf_bounded xhi)
-    | @ins_left c x y t1 t1new t2 xy ins =>
-      fun lo hi lox xhi b =>
-        use_node_bounded
-          b
-          (fun b1 b2 =>
-             let loy := bounds_le b1 in
-             let yhi := bounds_le b2 in
-             let bnew := f x t1 t1new ins lo y lox xy b1 in
-             node_bounded c bnew b2
-          )
-    | @ins_right c x y t1 t2 t2new yx ins =>
-      fun lo hi lox xhi b =>
-        use_node_bounded
-          b
-          (fun b1 b2 =>
-             let loy := bounds_le b1 in
-             let yhi := bounds_le b2 in
-             let bnew := f x t2 t2new ins y hi yx xhi b2 in
-             node_bounded c b1 bnew
-          )
-    | @ins_replace c x y t1 t2 eqv =>
-      fun _ _ _ _ b =>
-        use_node_bounded
-          b
-          (fun b1 b2 =>
-             And.use
-               eqv
-               (fun xy yx  =>
-                  node_bounded
-                    c
-                    (bounded_right_transitive b1 yx)
-                    (bounded_left_transitive b2 xy)
-               )
-          )
-    | @ins_rotation x t1 t2 t3 ins rot =>
-      fun lo hi lox xhi b =>
-        rotation_bounded
-          rot
-          (f x t1 t2 ins lo hi lox xhi b)
-    end.
-
-
-
-
-
-  Definition RBT: Type := {t:tree | is_Red_black t}.
-
-  Definition RBN: Type := {t:tree | exists h, RB_nearly0 h t}.
-
-  Theorem nearly_leaf_to_absurd:
-    forall (h:nat), RB_nearly0 h Leaf -> False.
-  Proof.
-    refine (
-      let f: forall h t, RB_nearly0 h t -> t = Leaf -> False :=
-          fun _ _ nrb =>
-            match nrb with
-              nearly _ _ _ _ =>
-              fun eq: Node _ _ _ _ = Leaf =>
-                _ (* inversion leads to contradiction *)
-            end
-      in
-      fun h nrb => f h Leaf nrb eq_refl
-    ).
-    inversion eq.
-  Qed.
-
-  Theorem nearly_node_to_rb:
-    forall (h:nat) (c:Color) (t1:tree) (x:S.t) (t2:tree),
-      RB_nearly0 h (Node c t1 x t2) ->
-      Red_black (S h) Black (Node Black t1 x t2).
-  Proof.
-    refine (
-        let f: forall h t c t1 x t2,
-            RB_nearly0 h t -> t = Node c t1 x t2 ->
-            Red_black (S h) Black (Node Black t1 x t2) :=
-            fun h t c t1 x t2 nrb =>
-              match nrb with
-                @nearly h2 ca ta z cb tb c3 rba rbb =>
-                fun eq => _
-          end
-        in
-        fun h c t1 x t2 nrb => f h (Node c t1 x t2) c t1 x t2 nrb eq_refl
-      ).
-    inversion eq as [ (eqc,eqt1,eqx,eqt2) ].
-    apply rb_black with (c1:=ca) (c2:=cb).
-    - rewrite <- eqt1; assumption.
-    - rewrite <- eqt2; assumption.
-  Qed.
-
-
-  Definition make_black (t:RBN): RBT.
-    refine (
-        match t with
-          exist _ t rbn =>
-          (match t with
-           | Leaf =>
-             let f: forall t, (exists h,RB_nearly0 h t) -> t = Leaf -> False :=
-                 fun t rbn =>
-                   match rbn with
-                     ex_intro _ h nrb =>
-                     match nrb with
-                       nearly x c3 rb1 rb2 =>
-                       fun eq => _ (* inversion leads to contradiction *)
-                     end
-                   end
-             in
-             fun rbn => match f Leaf rbn eq_refl with end
-           | Node c t1 x t2 =>
-             fun rbn =>
-               let t := Node Black t1 x t2 in
-               let rbt: exists h, Red_black h Black t :=
-                   match rbn with
-                     ex_intro _ h rb =>
-                     let q := @nearly_node_to_rb h c t1 x t2 rb in
-                     ex_intro _ (S h) q
-                   end
-               in
-               exist _ t rbt
-           end) rbn
-        end).
-    inversion eq.
-  Defined.
-
-
-
-
-  Definition make_black2 (t:tree): is_Nearly t -> RBT.
-    refine (
-        match t with
-        | Leaf =>
-          let f: forall t, (exists h,RB_nearly0 h t) -> t = Leaf -> False :=
-              fun t rbn =>
-                match rbn with
-                  ex_intro _ h nrb =>
-                  match nrb with
-                    nearly x c3 rb1 rb2 =>
-                    fun eq => _ (* inversion leads to contradiction *)
-                  end
-                end
-          in
-          fun rbn => match f Leaf rbn eq_refl with end
-        | Node c t1 x t2 =>
-          fun rbn =>
-            let t := Node Black t1 x t2 in
-            let rbt: exists h, Red_black h Black t :=
-                match rbn with
-                  ex_intro _ h rb =>
-                  let q := @nearly_node_to_rb h c t1 x t2 rb in
-                  ex_intro _ (S h) q
-                end
-            in
-            exist _ t rbt
-        end
-      ).
-    inversion eq.
-  Defined.
-
-
-  (*====================================*)
-  (** * Insertion *)
-  (*====================================*)
-
-
-
-
-  Definition Insert_result (x:S.t) (t:tree): Type :=
-    {u:tree | is_Red_black u /\ Inserted x t u}. (* inserted implies sorted *)
-
-  Definition Ins_red_balanced (x:S.t) (t u:tree): Prop :=
-    forall h, Red_black h Red t -> RB_nearly0 h u.
-
-  Definition Ins_black_balanced (x:S.t) (t u:tree): Prop :=
-    forall h, Red_black h Black t -> Red_black h (color u) u.
-
-  Definition Ins_balanced (x:S.t) (t u:tree): Prop :=
-    Ins_red_balanced x t u \/ Ins_black_balanced x t u.
-
-  Definition Ins_result (x:S.t) (t u:tree): Prop :=
-    Inserted x t u /\
-    Ins_balanced x t u.
-
-
-  Definition Black_son_inserted
-             (x:S.t) (t u v w:tree)
-    : Prop :=
-    (* t is a black tree and one of the sons of v. x has been inserted into t
-    and the result is u. Therefore u is sorted and balanced. The proposition
-    states that x is inserted into v resulting in w where w is nearly
-    balanced.*)
-    forall c h lo hi,
-      lo <= x ->
-      x <= hi ->
-      Inserted x t u ->
-      Bounded lo u hi ->
-      Red_black h c u ->
-      Inserted x v w /\ RB_nearly0 h w.
-
-  Definition Red_son_inserted
-             (x:S.t) (t u v w:tree)
-    : Prop :=
-    (* t is a red tree and one of the sons of v. x has been inserted into t
-    resulting in u. Therefore u is sorted, red and nearly balanced (maybe
-    fully balanced). The proposition states that x has been inserted into v
-    resulting in w where w is balanced. The color of w can be red or black. If
-    u is balanced then the color can stay black as the color of v. If u has a
-    red son and grandson then the blackness of v might have been pushed down
-    and w might be red.*)
-    forall h lo hi,
-      lo <= x ->
-      x <= hi ->
-      Inserted x t u ->
-      Bounded lo u hi ->
-      is_Node_red u ->
-      RB_nearly0 h u ->
-      Inserted x v w /\ exists c, Red_black (S h) c w.
-
-
-
-  (** ins: forall t, is_Red_black t -> Sorted t -> Ins_result x t u
-
-  'ins' gets a sorted redblack tree and returns an inserted and possibly
-  rebalanced tree.
-
-  Insertion into a node (t1 y' t2) either into the left or right son. 'ins t0
-  rb0 s0' returns Ins_result x' ta ua where ta is either t1 or t2.
-
-  There are two cases needing rebalancing:
-
-  a) u0 = N R (N R a x b) y c
-
-  b) u0 = N R a x (N R b y c)
-
-  Since is_Nearly u0, Ins_result x ta ua must be the case Ins_red_balanced x'
-  ta ua, i.e. ta must be red and the original tree (t1 y' t2) must be
-  black. All subtrees a b c have height h where h is the height of ta. The
-  other son of the original tree tb must have the same height. The rebalanced
-  trees are
-
-      N R (N B a x b) y (N B c y' tb) -- tb is the right son
-
-      N R (N B tb y' a) x (N B b y c) -- tb is the left son
-
-  The original tree has height 1+h and the rebalanced as well. Therefore we
-  can return Ins_black_balanced x' t u which is a valid Ins_result.
-
-  All the other cases don't need rebalancing. We have to prove this case by case.
-
-
-  This case is impossible, because x' has been inserted into t0.
-
-  The remaining case are nodes. After the rebalance cases there remain:
-
-  a) u0 = Leaf                          -- impossible, no insertion
-  b) u0 = N B a x b                     -- original black, balanced
-  c) u0 = N R Leaf x Leaf               -- insertion into empty tree
-  d) u0 = N R Leaf x (N B b y c)        -- impossible: neither nearly nor balanced
-  e) u0 = N R (N B a x b) y Leaf        -- impossible: neither nearly nor balanced
-  f) u0 = N R (N B a x b) y (N B c z d) -- balanced
-
-   *)
-
-  Theorem rebalance:
-    forall (x0:S.t) (t0 u0:tree),
-      is_Red_black t0 ->
-      Sorted t0 ->
-      Inserted x0 t0 u0 ->
-      Ins_balanced x0 t0 u0 ->
-      False.
-  Proof
-    fun x0 t0 u0 =>
-      match u0 with
-      | Node Red (Node Red a x b) y c => _
-      | Node Red a x (Node Red b y c) => _
-      | Leaf => _
-      | Node Black a x b => _
-      | Node Red Leaf x Leaf => _
-      | Node Red Leaf x (Node Black b y c) => _
-      | Node Red (Node Black a x b) y Leaf => _
-      | Node Red (Node Black a x b) y (Node Black c z d) => _
-      end.
-
-  Import Relation.
-
-  Definition insert
-             (x:S.t) (t:tree)
-    : is_Red_black t -> Sorted t -> Insert_result x t :=
-    let ins: forall t,
-        is_Red_black t -> Sorted t ->  {u | Ins_result x t u } :=
-        fix f t :=
-          match t with
-          | Leaf =>
-            fun rb s =>
-              let u := Node Red Leaf x Leaf in
-              exist
-                _ u
-                (conj
-                   (ins_leaf Red x)
-                   (or_intror
-                      (generalize_height
-                         (fun h => Red_black h Red u)
-                         rb_leaf
-                         (rb_red x rb_leaf rb_leaf)
-                       : forall h, Red_black h Black Leaf -> Red_black h Red u
-                       ))
-                 :Ins_result x Leaf u)
-          | Node c t1 y t2 =>
-            match S.compare3 x y with
-            | less_than xy =>
-              fun rb s =>
-                match f t1 (left_son_red_black rb) (left_son_sorted s) with
-                | exist _ u1 inv1 =>
-                  match c with
-                  | Red =>
-                    let u := Node Red u1 y t2 in
-                    exist
-                      _ u
-                      (_: Ins_result x _ u)
-                  | Black => _
-                  end
-                end
-            | equivalent xy yx =>_
-            | greater_than yx =>_
-            end
-          end
-    in
-    let mblack: forall u, Ins_result x t u -> Insert_result x t := _ in
-    fun rb s => Sigma.use (ins t rb s) (fun u p => mblack u p).
-End M1.
-
-
-
-
-
-
-
-(* ************* cpdt chlipala **************)
+(* ************ Left Leaning Red Black Tree **************)
 Module Make (S0:SORTABLE).
   Module S := Sortable_plus S0.
   Import S.Notations.
 
   Module Color.
-    Inductive t: Set := Red | Black.
+    Inductive t0: Set := Red | Black.
+
+    Definition t := t0.
+
+    Definition is_Red (c:t): Prop :=
+      match c with
+      | Red => True
+      | Black => False
+      end.
+
+    Definition is_Black (c:t): Prop :=
+      match c with
+      | Red => False
+      | Black => True
+      end.
+
+    Theorem red_equal_black {A:Type} (eq:Red=Black): A.
+    Proof
+      ex_falso (Equal.use eq is_Red I).
+
+    Theorem black_equal_red {A:Type} (eq:Black=Red): A.
+    Proof
+      red_equal_black (Equal.flip eq).
   End Color.
 
-  (* Invariant:
-     1. The black depth in both subtrees is the same.
-     2. A red parent has two black sons.
-   *)
 
 
 
-  Inductive t : Color.t -> nat -> Set :=
-  | Leaf :
-      t Color.Black 0
-  | Red_node :
-      forall n,
-        t Color.Black n ->
-        S.t ->
-        t Color.Black n ->
-        t Color.Red n
-  | Black_node :
-      forall c1 c2 n,
-        t c1 n ->
-        S.t ->
-        t c2 n ->
-        t Color.Black (S n).
+
+  Module BST := Binary_search_tree.Make S Color.
+  Import BST.
+  Import BST.BT.
+
+  Definition color (t:Tree.t): Color.t :=
+    match t with
+    | Tree.Leaf => Color.Black
+    | Tree.Node c _ _ _ => c
+    end.
 
 
-  Extraction t.
-  (* A nearly red black tree might have a root node with arbitrary colored
-     sons. The black-height invariant is valid and the sons are valid red
-     black trees of the same black depth. *)
-  Inductive nearly: nat -> Set :=
-  | Nearly:
-      forall c1 c2 n,
-        t c1 n ->
-        S.t ->
-        t c2 n ->
-        nearly n.
 
 
-  (*
-    Inductive sigT (A : Type) (T : A -> Type) : Type :=
-    | existT :
-        forall x : A,
-            T x ->
-            {x : A & T x}.
 
-     T is a dependend type. It maps a value of type A into the type T a.
+  Module Red_black.
+    Inductive R: nat -> Color.t -> Tree.t -> Prop :=
+    | leaf: R 0 Color.Black Tree.Leaf
+    | red:
+        forall h t1 x t2,
+          R h Color.Black t1 ->
+          R h Color.Black t2 ->
+          R h Color.Red (Tree.Node Color.Red t1 x t2)
+    | black:
+        forall h c1 t1 x c2 t2,
+          R h c1 t1 ->
+          R h c2 t2 ->
+          R (S h) Color.Black (Tree.Node Color.Black t1 x t2).
 
-     {x: A & T} is a notation for sigT (fun x : A => T)
-   *)
-  (*Definition balance1
-             (n:nat) (a:nearly n)
-             (e:S.t) (c2:Color.t)
-             (b:t c2 n)
-    : {c:Color.t & t c (S n)} :=
-    _.*)
+    Inductive P (t:Tree.t): Prop :=
+      make: forall h c, R h c t -> P t.
 
+    Theorem color_correct {h:nat} {c:Color.t} {t:Tree.t} (rb:R h c t)
+      : c = color t.
+    Proof
+      match rb in R h c t return c = color t with
+      | leaf => eq_refl
+      | red x rb1 rb2 => eq_refl
+      | black x rb1 rb2 => eq_refl
+      end.
+
+    Theorem color_unique {h1 h2:nat} {c1 c2:Color.t} {t:Tree.t}
+            (rb1:R h1 c1 t) (rb2:R h2 c2 t): c1 = c2.
+    Proof
+      Equal.join (color_correct rb1) (Equal.flip (color_correct rb2)).
+
+    Theorem pull_color:
+      forall (h:nat) (c1 c2:Color.t) (x:S.t) (u v:Tree.t),
+        R h c1 (Tree.Node c2 u x v) ->
+        R h c2 (Tree.Node c2 u x v).
+    Proof
+      fun h c1 c2 x u v rb =>
+        Equal.use
+          (color_correct rb: c1 = c2)
+          (fun c => R _ c _)
+          rb.
+
+
+    Fixpoint black_height (t:Tree.t): nat :=
+      match t with
+      | Tree.Leaf => 0
+      | Tree.Node Color.Black t1 _ _ => S (black_height t1)
+      | Tree.Node Color.Red t1 _ _  => black_height t1
+      end.
+
+    Theorem black_height_correct:
+        forall (h:nat) (c:Color.t) (t:Tree.t),
+          R h c t ->
+          h = black_height t.
+    Proof
+      fix f h c t rb :=
+      match rb with
+      | leaf => eq_refl
+      | red x rb1 rb2 =>
+        f _ _ _ rb1
+      | black x rb1 rb2 =>
+        Equal.inject (f _ _ _ rb1) S
+      end.
+
+    Theorem black_height_unique:
+      forall (h1 h2:nat) (c1 c2:Color.t) (t:Tree.t),
+        R h1 c1 t ->
+        R h2 c2 t ->
+        h1 = h2.
+    Proof
+      fun h1 h2 c1 c2 t rb1 rb2 =>
+        Equal.join
+          (black_height_correct rb1)
+          (Equal.flip (black_height_correct rb2)).
+
+
+    Theorem use_red_node0:
+      forall (A:Prop) h t u x v,
+        R h Color.Red t ->
+        t = Tree.Node Color.Red u x v ->
+        (R h Color.Black u ->
+         R h Color.Black v ->
+         R h Color.Red (Tree.Node Color.Red u x v) ->
+         A) ->
+        A.
+    Proof
+      fix f A h t u x v rb :=
+      match rb with
+      | leaf =>
+        fun eq =>
+          Tree.leaf_equal_node eq
+      | red x rb1 rb2 =>
+        fun eq f =>
+          Tree.use_node_equal
+            eq
+            (fun ceq xeq ueq veq =>
+               let rbu := Equal.use ueq _ rb1 in
+               let rbv := Equal.use veq _ rb2 in
+               let rbt :=
+                   Equal.use xeq (fun x => R _ _ (Tree.Node _ _ x _))
+                             (red x rbu rbv) in
+               f rbu rbv rbt)
+      | black x rb1 rb2 =>
+        fun eq f =>
+          Tree.use_node_equal
+            eq
+            (fun ceq _ _ _ => Color.black_equal_red ceq)
+      end.
+
+
+    Theorem use_black_node0:
+      forall (A:Prop) h t u x v,
+        R h Color.Black t ->
+        t = Tree.Node Color.Black u x v ->
+        (forall h cu cv,
+            R h cu u ->
+            R h cv v ->
+            R (S h) Color.Black (Tree.Node Color.Black u x v) ->
+            A) ->
+        A.
+    Proof
+      fix f A h t u x v rb :=
+      match rb with
+      | leaf =>
+        fun eq => Tree.leaf_equal_node eq
+      | red x rb1 rb2 =>
+        fun eq f =>
+          Tree.use_node_equal
+            eq
+            (fun ceq _ _ _ => Color.red_equal_black ceq)
+      | black x rb1 rb2 =>
+        fun eq f =>
+          Tree.use_node_equal
+            eq
+            (fun ceq xeq ueq veq =>
+               let rbu := Equal.use ueq _ rb1 in
+               let rbv := Equal.use veq _ rb2 in
+               let rbt :=
+                   Equal.use xeq (fun x => R _ _ (Tree.Node _ _ x _))
+                             (black x rbu rbv) in
+               f _ _ _ rbu rbv rbt)
+
+      end.
+
+
+    Theorem use_red_node:
+      forall (A:Prop) h u x v,
+        R h Color.Red (Tree.Node Color.Red u x v) ->
+        (R h Color.Black u ->
+         R h Color.Black v ->
+         R h Color.Red (Tree.Node Color.Red u x v) ->
+         A) ->
+        A.
+    Proof
+      fun A h u x v rbt f =>
+        use_red_node0 rbt eq_refl f.
+
+
+
+    Theorem use_black_node:
+      forall (A:Prop) h u x v,
+        R h Color.Black (Tree.Node Color.Black u x v) ->
+        (forall h cu cv,
+            R h cu u ->
+            R h cv v ->
+            R (S h) Color.Black (Tree.Node Color.Black u x v) ->
+            A) ->
+        A.
+    Proof
+      fun A h u x v rbt f =>
+        use_black_node0 rbt eq_refl f.
+
+    Theorem use_left_red0:
+      forall (A:Prop) h h0 c t u x v,
+        R h c t ->
+        t = Tree.Node c u x v ->
+        R h0 Color.Red u ->
+        (forall h cv,
+            R h Color.Red u ->
+            R h cv v ->
+            R (S h) c (Tree.Node c u x v) ->
+            A) ->
+        A.
+    Proof
+      fun A h h0 c t u x v rbt =>
+        match rbt with
+        | leaf =>
+          fun eq => Tree.leaf_equal_node eq
+        | red x rb1 rb2 =>
+          fun eq rbu f =>
+            Tree.use_node_equal
+              eq
+              (fun eqc eqx eq1 eq2 =>
+                 let rb1 := Equal.use eq1 (Red_black.R _ _) rb1 in
+                 Color.black_equal_red (color_unique rb1 rbu))
+        | black x rb1 rb2 =>
+          fun eq rbu f =>
+            Tree.use_node_equal
+              eq
+              (fun eqc eqx eq1 eq2 =>
+                 let rb1 := Equal.use eq1 (Red_black.R _ _) rb1 in
+                 let heq: _ = h0 := black_height_unique rb1 rbu in
+                 let rbv :=
+                     Equal.use2 heq eq2 (fun h t => Red_black.R h _ t) rb2 in
+                 f _ _ rbu rbv
+                   (Equal.use
+                      eqx (fun x => R _ _ (Tree.Node _ _ x _))
+                      (black x rbu rbv)))
+        end.
+
+
+    Theorem use_left_red:
+      forall (A:Prop) h h0 c1 c2 u x v,
+        R h c1 (Tree.Node c2 u x v) ->
+        R h0 Color.Red u ->
+        (forall h cv,
+            R h Color.Red u ->
+            R h cv v ->
+            R (S h) c2 (Tree.Node c2 u x v) ->
+            A) ->
+        A.
+    Proof
+      fun A h h0 c1 c2 u x v rbt rbu f =>
+        let rbt := pull_color rbt in
+        use_left_red0 rbt eq_refl rbu f.
+  End Red_black.
+
+
+
+
+
+  Module Red_black_sorted.
+    Inductive P (t:Tree.t): Prop :=
+      make:
+        forall h c lo hi,
+          Red_black.R h c t ->
+          Sorted.R lo t hi ->
+          P t.
+
+
+    Theorem use_black_node:
+      forall (A:Prop) (x:S.t) (u v: Tree.t),
+        P (Tree.Node Color.Black u x v) ->
+        (forall h cu cv lo hi,
+            Red_black.R h cu u ->
+            Red_black.R h cv v ->
+            Red_black.R (S h) Color.Black (Tree.Node Color.Black u x v) ->
+            lo <= x ->
+            x <= hi ->
+            Sorted.R lo u x ->
+            Sorted.R x  v hi ->
+            Sorted.R lo (Tree.Node Color.Black u x v) hi ->
+            A) ->
+        A.
+    Proof
+      fun A x u v p =>
+        match p with
+          make rbt st =>
+          Red_black.use_black_node
+            (Red_black.pull_color rbt)
+            (fun h cu cv rbu rbv rbt f =>
+               Sorted.use_node
+                 st
+                 (fun lox xhi su sv =>
+                    f h cu cv _ _ rbu rbv rbt lox xhi su sv st))
+        end.
+
+
+    Theorem use_red_node:
+      forall (A:Prop) (x:S.t) (u v: Tree.t),
+        P (Tree.Node Color.Red u x v) ->
+        (forall h lo hi,
+            Red_black.R h Color.Black u ->
+            Red_black.R h Color.Black v ->
+            Red_black.R h Color.Red (Tree.Node Color.Red u x v) ->
+            lo <= x ->
+            x <= hi ->
+            Sorted.R lo u x ->
+            Sorted.R x v hi ->
+            Sorted.R lo (Tree.Node Color.Red u x v) hi ->
+            A) ->
+        A.
+    Proof
+      fun A x u v p =>
+        match p with
+          make rbt st =>
+          Red_black.use_red_node
+            (Red_black.pull_color rbt)
+            (fun rbu rbv rbt f =>
+               Sorted.use_node
+                 st
+                 (fun lox xhi su sv =>
+                    f _ _ _ rbu rbv rbt lox xhi su sv st))
+        end.
+
+
+
+    Theorem use_node:
+      forall (A:Prop) c u x v,
+        P (Tree.Node c u x v) ->
+        (forall h h0 cu cv lo hi,
+            Red_black.R h0 cu u ->
+            Red_black.R h0 cv v ->
+            Red_black.R h c (Tree.Node c u x v) ->
+            lo <= x ->
+            x <= hi ->
+            Sorted.R lo u x ->
+            Sorted.R x v hi ->
+            Sorted.R lo (Tree.Node c u x v) hi ->
+            A) ->
+        A.
+    Proof
+      fun A c =>
+        match c with
+        | Color.Red =>
+          fun u x v p f =>
+            use_red_node
+              p
+              (fun h lo hi rbu rbv rbt lox xhi su sv st =>
+                 f _ _ _ _ _ _ rbu rbv rbt lox xhi su sv st)
+        | Color.Black =>
+          fun u x v p f =>
+            use_black_node
+              p
+              (fun h cu cv lo hi rbu rbv rbt lox xhi su sv st =>
+                 f _ _ _ _ _ _ rbu rbv rbt lox xhi su sv st)
+        end.
+
+
+
+    Theorem use_node1:
+      forall (A:Prop) (c:Color.t) (x:S.t) (u v:Tree.t),
+        P (Tree.Node c u x v) ->
+        (P u -> P v -> A) ->
+        A.
+    Proof
+      fun A c x u v p =>
+        use_node
+          p
+          (fun h h0 cu cv lo hi rbu rbv rbt lox xhi su sv st f =>
+             f (make rbu su) (make rbv sv)).
+
+
+    Theorem left_son:
+      forall (c:Color.t) (x:S.t) (u v:Tree.t),
+        P (Tree.Node c u x v) -> P u.
+    Proof
+      fun c x u v p =>
+        use_node1
+          p
+          (fun pu pv => pu).
+
+
+
+    Theorem use_left_red:
+      forall (A:Prop) (h:nat) (c:Color.t) (x:S.t) (u v: Tree.t),
+        P (Tree.Node c u x v) ->
+        Red_black.R h Color.Red u ->
+        (forall h cv lo hi,
+            Red_black.R h Color.Red u ->
+            Red_black.R h cv v ->
+            Red_black.R (S h) c (Tree.Node c u x v) ->
+            lo <= x ->
+            x <= hi ->
+            Sorted.R lo u x ->
+            Sorted.R x v hi ->
+            Sorted.R lo (Tree.Node Color.Black u x v) hi ->
+            A) ->
+        A.
+    Proof
+      fun A h c x u v rbst =>
+        match rbst with
+          make rbt_0 st =>
+          fun rbu f =>
+            Red_black.use_left_red
+              (Red_black.pull_color rbt_0) rbu
+              (fun cv rbu rbv rbt =>
+                 let st := Sorted.change_extra Color.Black st in
+                 Sorted.use_node
+                   st
+                   (fun lox xhi s1 s2 =>
+                      f _ _ _ _ rbu rbv rbt lox xhi s1 s2 st))
+        end.
+  End Red_black_sorted.
+
+
+  Module Insertion.
+    Module Red_black_inserted.
+      Inductive R (e:S.t) (t u: Tree.t): Prop :=
+        make:
+          forall h c,
+            Red_black.R h c u ->
+            Inserted.R e t u ->
+            R e t u.
+    End Red_black_inserted.
+
+
+    Definition result (e:S.t) (t:Tree.t): Type :=
+      {u:Tree.t | Red_black_inserted.R e t u}.
+
+    Module Red_red.
+      Inductive R
+                (e:S.t) (t:Tree.t)
+                (a:Tree.t) (x:S.t) (b:Tree.t) (y:S.t) (c:Tree.t): Prop :=
+        make:
+        forall h,
+          Red_black.R h Color.Red t ->
+          Red_black.R h Color.Black a ->
+          Red_black.R h Color.Black b ->
+          Red_black.R h Color.Black c ->
+          Inserted.R e t (Tree.Node Color.Red (Tree.Node Color.Red a x b) y c) ->
+          R e t a x b y c.
+    End Red_red.
+
+    Module Red.
+      Inductive R (e:S.t) (t:Tree.t) (a:Tree.t) (x:S.t) (b:Tree.t): Prop :=
+        make:
+          forall h c,
+            Red_black.R h c t ->
+            Red_black.R h Color.Black a ->
+            Red_black.R h Color.Black b ->
+            Inserted.R e t (Tree.Node Color.Red a x b) ->
+            R e t a x b.
+    End Red.
+
+    Module Black.
+      Inductive R (e:S.t) (t:Tree.t) (a:Tree.t) (x:S.t) (b:Tree.t): Prop :=
+        make:
+          forall h ca cb,
+            Red_black.R (S h) Color.Black t ->
+            Red_black.R h ca a ->
+            Red_black.R h cb b ->
+            Inserted.R e t (Tree.Node Color.Black a x b) ->
+            R e t a x b.
+    End Black.
+
+    (** If we have a red red violation we just repaint the root node black. *)
+(**<<
+                yR                                    yB
+            xR                                    xR
+         a     b    c                          a     b    c
+>>*)
+    Theorem inserted_of_red_red:
+      forall e t a x b y c,
+        Red_red.R e t a x b y c ->
+        Red_black_inserted.R
+          e t
+          (Tree.Node
+             Color.Black
+             (Tree.Node Color.Red a x b)
+             y
+             c).
+    Proof
+      fun e t a x b y c rr =>
+        match rr with
+          Red_red.make rbt rba rbb rbc ins =>
+          Red_black_inserted.make
+            (Red_black.black y (Red_black.red x rba rbb) rbc)
+            (Inserted.change_extra Color.Black ins)
+        end.
+
+    (** A red node is already valid. Nothing to be done. *)
+    Theorem inserted_of_red:
+      forall e t a x b,
+        Red.R e t a x b ->
+        Red_black_inserted.R
+          e t
+          (Tree.Node Color.Red a x b).
+    Proof
+      fun e t a x b r =>
+        match r with
+          Red.make _ rba rbb ins =>
+          Red_black_inserted.make (Red_black.red _ rba rbb) ins
+        end.
+
+    (** A black node is already valid. Nothing to be done. *)
+    Theorem inserted_of_black:
+      forall e t a x b,
+        Black.R e t a x b ->
+        Red_black_inserted.R
+          e t
+          (Tree.Node Color.Black a x b).
+    Proof
+      fun e t a x b black =>
+        match black with
+          Black.make _ rba rbb ins =>
+          Red_black_inserted.make (Red_black.black _ rba rbb) ins
+        end.
+Check Inserted.change_left_extra.
+
+
+    (** We have the situation: *)
+(**<<
+            yn           where u1            yR
+        t1R   t2                          xR     c
+                                        a    b
+    which we insert as the new left subtree
+          ynB                                 yR
+       yR     t2     rotate right         xB     ynB
+     xR   c          repaint x           a  b   c  t2
+    a  b
+>>*)
+    (** t2 has the same black height as [a,b,c]. The parent of t1 and t2 must
+    be black because t1 is red. Therefore the resulting tree can have one
+    black height level more than t1, a, b and c.*)
+    Theorem red_of_left_red_red:
+      forall e cn t1 yn t2 a x b y c,
+        Red_black_sorted.P (Tree.Node cn t1 yn t2) ->
+        e <= yn ->
+        Red_red.R e t1 a x b y c ->
+        Red.R e
+              (Tree.Node cn t1 yn t2)
+              (Tree.Node Color.Black a x b)
+              y
+              (Tree.Node Color.Black c yn t2).
+    Proof
+      fun e cn t1 yn t2 a x b y c rbs eyn rr =>
+        match rr with
+          Red_red.make rbt1_0 rba rbb rbc ins1 =>
+          Red_black_sorted.use_left_red
+            rbs
+            rbt1_0
+            (fun h ct2 lo hi rbt1 rbt2 rbt lo_yn yn_hi st1 st2 st =>
+               let insu :=
+                   Inserted.change_left_extra
+                     Color.Black
+                     (Inserted.rotate_right
+                        (Inserted.left
+                           cn Color.Black eyn st1 st2 ins1))
+               in
+               let heq: _ = h := Red_black.black_height_unique rbt1_0 rbt1 in
+               let P t h := Red_black.R h _ t in
+               Red.make
+                 rbt
+                 (Red_black.black
+                    x
+                    (Equal.use heq (P a) rba)
+                    (Equal.use heq (P b) rbb))
+                 (Red_black.black
+                    yn
+                    (Equal.use heq (P c) rbc)
+                    rbt2)
+                 insu)
+        end.
+
+
+    Theorem red_red_of_left_red:
+      forall e t1 yn t2 a x b,
+        Red_black_sorted.P (Tree.Node Color.Red t1 yn t2) ->
+        e <= yn ->
+        Red.R e t1 a x b ->
+        Red_red.R
+          e (Tree.Node Color.Red t1 yn t2)
+          a x b yn t2.
+    Proof
+      fun e t1 yn t2 a x b rbst e_yn r =>
+        match r with
+          Red.make rbt1_0 rba rbb ins1 =>
+          Red_black_sorted.use_red_node
+            rbst
+            (fun h lo hi rbt1 rbt2 rbt lo_yn yn_hi st1 st2 st =>
+               let insu :=
+                   Inserted.left
+                     Color.Red Color.Red e_yn st1 st2 ins1 in
+               let heq: _ = h := Red_black.black_height_unique rbt1_0 rbt1 in
+               let P t h := Red_black.R h Color.Black t in
+               Red_red.make
+                 rbt
+                 (Equal.use heq (P a) rba)
+                 (Equal.use heq (P b) rbb)
+                 rbt2
+                 insu)
+        end.
+
+    Theorem black_of_left_red:
+      forall e t1 yn t2 a x b,
+        Red_black_sorted.P (Tree.Node Color.Black t1 yn t2) ->
+        e <= yn ->
+        Red.R e t1 a x b ->
+        Black.R
+          e (Tree.Node Color.Black t1 yn t2)
+          (Tree.Node Color.Red a x b)
+          yn
+          t2.
+    Proof
+      fun e t1 yn t2 a x b rbst e_yn red =>
+        match red with
+          Red.make rbt1_0 rba rbb ins1 =>
+          Red_black_sorted.use_black_node
+            rbst
+            (fun h ct1 ct2 lo hi rbt1 rbt2 rbt lo_yn yn_hi st1 st2 st =>
+               let heq: _ = h := Red_black.black_height_unique rbt1_0 rbt1 in
+               let P t h := Red_black.R h _ t in
+               Black.make
+                 rbt
+                 (Red_black.red
+                    x
+                    (Equal.use heq (P a) rba)
+                    (Equal.use heq (P b) rbb))
+                 rbt2
+                 (Inserted.left
+                    Color.Black Color.Black e_yn st1 st2 ins1)
+            )
+        end.
+
+
+    Theorem black_of_left_black:
+      forall e t1 yn t2 a x b,
+        Red_black_sorted.P (Tree.Node Color.Black t1 yn t2) ->
+        e <= yn ->
+        Black.R e t1 a x b ->
+        Black.R
+          e (Tree.Node Color.Black t1 yn t2)
+          (Tree.Node Color.Black a x b)
+          yn
+          t2.
+    Proof
+      fun e t1 yn t2 a x b rbst e_yn black =>
+        match black with
+          Black.make rbt1_0 rba rbb ins1 =>
+          Red_black_sorted.use_black_node
+            rbst
+            (fun h ct1 ct2 lo hi rbt1 rbt2 rbt lo_yn yn_hi st1 st2 st =>
+               let heq: _ = h := Red_black.black_height_unique rbt1_0 rbt1 in
+               Black.make
+                 rbt
+                 (Equal.use
+                    heq (fun h => Red_black.R h _ _)
+                    (Red_black.black x rba rbb))
+                 rbt2
+                 (Inserted.left Color.Black Color.Black e_yn st1 st2 ins1)
+            )
+        end.
+
+
+
+    Theorem red_of_left_black:
+      forall e t1 yn t2 a x b,
+        Red_black_sorted.P (Tree.Node Color.Red t1 yn t2) ->
+        e <= yn ->
+        Black.R e t1 a x b ->
+        Red.R
+          e (Tree.Node Color.Red t1 yn t2)
+          (Tree.Node Color.Black a x b)
+          yn
+          t2.
+    Proof
+      fun e t1 yn t2 a x b rbst e_yn black =>
+        match black with
+          Black.make rbt1_0 rba rbb ins1 =>
+          Red_black_sorted.use_red_node
+            rbst
+            (fun h lo hi rbt1 rbt2 rbt lo_yn yn_hi st1 st2 st =>
+               let heq: _ = h := Red_black.black_height_unique rbt1_0 rbt1 in
+               Red.make
+                 rbt
+                 (Equal.use
+                    heq (fun h => Red_black.R h _ _)
+                    (Red_black.black x rba rbb))
+                 rbt2
+                 (Inserted.left Color.Red Color.Red e_yn st1 st2 ins1)
+            )
+        end.
+
+
+
+    Inductive result0 (e:S.t) (t:Tree.t): Set :=
+    | Red_red:
+        forall a x b y c,
+          Red_red.R e t a x b y c ->
+          result0 e t
+    | Red:
+        forall a x b,
+          Red.R e t a x b ->
+          result0 e t
+    | Black:
+        forall a x b,
+          Black.R e t a x b ->
+          result0 e t.
+
+    Definition insert (e:S.t) (t:Tree.t) (rbs:Red_black_sorted.P t): result e t :=
+      let insert0:
+            forall t,
+              Red_black_sorted.P t -> result0 e t :=
+          fix insert0 t :=
+            match t with
+
+            | Tree.Leaf =>
+              fun _ =>
+                let rbl := Red_black.leaf in
+                Red (Red.make rbl rbl rbl (Inserted.leaf Color.Red e))
+
+            | Tree.Node cn t1 yn t2 =>
+
+              match S.compare3 e yn with
+
+              | Relation.less_than e_yn =>
+
+                fun rbs =>
+                  (match insert0 t1 (Red_black_sorted.left_son rbs), cn with
+                   | Red_red red_red, _ =>
+
+                     fun _ => Red (red_of_left_red_red rbs e_yn red_red)
+
+                   | Red red, Color.Red =>
+
+                     fun rbs => Red_red (red_red_of_left_red rbs e_yn red)
+
+                   | Red red, Color.Black =>
+
+                     fun rbs => Black (black_of_left_red rbs e_yn red)
+
+                   | Black black, Color.Black =>
+
+                     fun rbs => Black (black_of_left_black rbs e_yn black)
+
+                   | Black black, Color.Red =>
+
+                     fun rbs => Red (red_of_left_black rbs e_yn black)
+                  end) rbs
+
+              | Relation.equivalent e_yn yn_e =>
+
+                match cn with
+
+                | Color.Red =>
+                  fun rbst =>
+                    let red :=
+                        Red_black_sorted.use_red_node
+                          rbst
+                          (fun h lo hi rbt1 rbt2 rbt lo_yn yn_hi st1 st2 st =>
+                             Red.make
+                               rbt rbt1 rbt2
+                               (Inserted.replace
+                                  Color.Red Color.Red
+                                  (conj e_yn yn_e) st1 st2))
+                    in
+                    Red red
+                | Color.Black =>
+
+                  fun rbst =>
+                    let black :=
+                        Red_black_sorted.use_black_node
+                          rbst
+                          (fun h ct1 ct2 lo hi rbt1 rbt2 rbt
+                               lo_yn yn_hi st1 st2 st =>
+                             Black.make
+                               rbt rbt1 rbt2
+                               (Inserted.replace
+                                  Color.Black Color.Black
+                                  (conj e_yn yn_e) st1 st2))
+                    in
+                    Black black
+                end
+
+              | Relation.greater_than yn_e =>
+                _
+              end
+            end
+      in
+      match insert0 t rbs with
+      | Red_red rr =>
+        exist _ _ (inserted_of_red_red rr)
+      | Red r =>
+        exist _ _ (inserted_of_red r)
+      | Black b =>
+        exist _ _ (inserted_of_black b)
+      end.
+  End Insertion.
 End Make.
